src/Rupicola/Examples/Utf8/Utils.v
@@ -38,34 +38,41 @@ Definition byte_of_fin_lt {n} (Hle: (n <= 256)%nat) (f: Fin.t n) : byte :=
                    eauto using Nat.lt_irrefl, Nat.le_lt_trans, Nat.lt_le_trans)
   end eq_refl.
 
-Lemma word_of_byte_of_fin {n} H (f: Fin.t n):
-  word_of_byte (byte_of_fin_lt H f) =
-  word.of_Z (word := word) (Z.of_nat (proj1_sig (Fin.to_nat f))).
-Proof.
-  unfold byte_of_fin_lt.
-  destruct Fin.to_nat as (bn & Hf).
-  generalize (eq_refl (Byte.of_nat bn)).
-  destruct (Byte.of_nat bn) as [b|] at 2 3;
-    cbn -[word.of_Z]; intros Hb.
-  - apply Byte.to_of_nat in Hb; subst bn.
-    rewrite Byte.to_nat_via_N, N_nat_Z; reflexivity.
-  - destruct Nat.lt_irrefl.
-Qed.
-
 Lemma Fin_to_nat_lt {n} (f: Fin.t n) m:
   (n <= m)%nat -> (proj1_sig (Fin.to_nat f) < m)%nat.
 Proof. intros; pose proof proj2_sig (Fin.to_nat f); simpl in *; lia. Qed.
-
-Lemma word_of_byte_sru_lt b:
-  (Z.to_nat (word.unsigned (word.sru (word := word) (word_of_byte b) (word.of_Z 3))) < 32)%nat .
-Proof.
-  pose proof word.unsigned_range (word.sru (word_of_byte b) (word.of_Z 3)).
-  apply (Z2Nat.inj_lt _ (Z.of_nat 32)); [lia..|].
-  rewrite word.unsigned_sru_shamtZ, Z.shiftr_div_pow2 by lia.
-  pose proof word.word_of_byte_range b; apply Z.div_lt_upper_bound; lia.
-Qed.
 
 Instance Convertible_Fin_byte {n} (Hle: (n <= 256)%nat) : Convertible (Fin.t n) byte :=
   byte_of_fin_lt Hle.
 Instance Convertible_Fin_byte_5: Convertible (Fin.t 5) byte :=
   Convertible_Fin_byte (n := 5) ltac:(lia).
+
+Section __.
+  Context {width: Z} {BW: Bitwidth width} {word: word.word width} {mem: map.map word byte}.
+  Context {word_ok : word.ok word} {mem_ok : map.ok mem}.
+
+  Lemma word_of_byte_of_fin {n} H (f: Fin.t n):
+    word_of_byte (byte_of_fin_lt H f) =
+      word.of_Z (word := word) (Z.of_nat (proj1_sig (Fin.to_nat f))).
+  Proof.
+    unfold byte_of_fin_lt.
+    destruct Fin.to_nat as (bn & Hf).
+    generalize (eq_refl (Byte.of_nat bn)).
+    destruct (Byte.of_nat bn) as [b|] at 2 3;
+      cbn -[word.of_Z]; intros Hb.
+    - apply Byte.to_of_nat in Hb; subst bn.
+      rewrite Byte.to_nat_via_N, N_nat_Z; reflexivity.
+    - destruct Nat.lt_irrefl.
+  Qed.
+
+  Lemma word_of_byte_sru_lt b:
+    (Z.to_nat (word.unsigned (word.sru (word := word) (word_of_byte b) (word.of_Z 3))) < 32)%nat .
+  Proof.
+    pose proof width_at_least_32 as H32.
+    pose proof Z.pow_le_mono_r 2 _ _ ltac:(lia) H32.
+    pose proof word.unsigned_range (word.sru (word_of_byte b) (word.of_Z 3)).
+    apply (Z2Nat.inj_lt _ (Z.of_nat 32)); [lia..|].
+    rewrite word.unsigned_sru_shamtZ, Z.shiftr_div_pow2 by lia.
+    pose proof word.word_of_byte_range b; apply Z.div_lt_upper_bound; lia.
+  Qed.
+End __.
